gens

generic/GenericSoundness.ec
@@ -28,7 +28,7 @@ module SoundnessAmp(P: MaliciousProver, V: HonestVerifier) = {
     var i : int;
     i <- 0;
     accept <- true; 
-    while(i <= N /\ accept) {  
+    while(i < N /\ accept) {  
       accept <@ Soundness(P,V).run(stat);
       i <- i + 1;
     } 
@@ -45,49 +45,48 @@ clone import WhileNotBProc as WNBP with type rt <- bool,
 
 section.
 
+op soundness_error : statement -> real.
+
 declare module P <: MaliciousProver {-M, -HV}.
 
-(* are these needed? after all we are proving <= probability *)
 declare axiom verify_ll : islossless HV.verify.
 declare axiom challenge_ll : islossless HV.challenge.
 declare axiom response_ll : islossless P.response.
 declare axiom commitment_ll : islossless P.commitment.
 
-op deltoid : real.
-
 declare axiom soundness &n statement:
     ! in_language soundness_relation statement =>
      Pr[Soundness(P,HV).run(statement) @ &n : res]
-         <= deltoid.
+         <= soundness_error statement.
 
 lemma soundness_seq &m statement n:
     ! in_language soundness_relation statement =>
-     0 <= n =>
+     1 <= n =>
      Pr[SoundnessAmp(P,HV).run(statement, n) @ &m : res]
-       <= deltoid ^ (n + 1).
+       <= (soundness_error statement) ^ n.
 proof.
 move => nil nz.
-have phs : phoare[ Soundness(P,HV).run : arg = (statement) ==> res ] <= deltoid.
+have phs : phoare[ Soundness(P,HV).run : arg = statement ==> res ] <= (soundness_error statement).
 bypr. move => &m0 H. 
 rewrite H. simplify. apply soundness.  assumption.
 have ->: Pr[SoundnessAmp(P, HV).run(statement, n) @ &m : res]    
- = Pr[ M(Soundness(P,HV)).whp((statement), fun x => !x,1,n+1, true) @ &m :  res ].
-byequiv (_: ={glob P, glob HV} /\  arg{1} = (statement, n) /\ arg{2} = ((statement), fun x => !x,1,n+1, true)  ==> _).  
+ = Pr[ M(Soundness(P,HV)).whp((statement), fun x => !x,1,n, true) @ &m :  res ].
+byequiv (_: ={glob P, glob HV} /\  arg{1} = (statement, n) /\ arg{2} = ((statement), fun x => !x,1,n, true)  ==> _).  
 proc.   sp.
-while (i{1} + 1 = M.c{2} /\ N{1} + 1 = e{2} /\ accept{1} = !MyP{2} r{2} /\ ={glob P, glob HV}
+while (i{1} + 1 = M.c{2} /\ N{1}  = e{2} /\ accept{1} = !MyP{2} r{2} /\ ={glob P, glob HV}
   /\ (i{2}, MyP{2}, s{2}, e{2}) =
-  ((stat{1}), fun (x : bool) => !x, 1, N{1}+1)  ).
+  ((stat{1}), fun (x : bool) => !x, 1, N{1})  ).
 wp.  call (_: ={glob P, glob HV}).
 sim. skip. progress. smt. smt.
 skip. progress.  smt. smt.
 auto.  auto.
 byphoare (_: arg = ((statement), fun (x : bool) => !x,
-                                       1, n + 1, true) ==> _).
+                                       1, (n - 1) + 1, true) ==> _).
 apply (asdsadq_le (Soundness(P,HV))). 
 proc.
 call verify_ll. call response_ll. call challenge_ll. call commitment_ll. skip. auto.
-apply phs. auto. 
-auto. auto. auto.
+apply phs. auto.   smt.
+auto. auto. 
 qed.
 
 end section.
